$$
\begin{aligned}
&\left(\sqrt{3+\sqrt5}+\sqrt{3-\sqrt5}\right)^2=10
\\
\text {Solution 1:} \\
&3+\sqrt5 \\
=&\frac{1}{2}(6+2\sqrt5) \\
=&\frac{1}{2}[(\sqrt5)^2+2\sqrt5+1^2] \\
=&\frac{1}{2}(\sqrt5+1)^2 \\
\\

&3-\sqrt5 \\
=&\frac{1}{2}(\sqrt5-1)^2 \\
\\
LHS=&\left(\sqrt{\frac{1}{2}(\sqrt5+1)^2}+\sqrt{\frac{1}{2}(\sqrt5-1)^2}\right)^2 \\
=&\frac{1}{2}(2\sqrt5)^2 \\
=&10 \\
\therefore LHS=&RHS \\
\\
\text {Solution 2:}\\
LHS=&3+\sqrt5+3-\sqrt5+2\sqrt{(3+\sqrt5)(3-\sqrt5)} \\
=&6+2\sqrt4 \\
=&10
\end{aligned}
$$


