---
mindmap-plugin: basic
---

# Topic 1-Algebraic expressions

## Overview - Learning Goals

### Identities: Know and be able to use the following formulas

#### Perfect square binomials

##### $(a+b)^2=a^2+2ab+b^2$

##### $(a-b)^2=a^2-2ab+b^2$

#### Difference of squares

##### $a^2-b^2=(a+b)(a-b)$

#### Trinomial Square

##### $(a+b+c)^2=a^2+b^2+c^2+2ab+2bc+2ac$

##### $(a+b-c)^2=a^2+b^2+c^2+2ab-2bc-2ac$

##### $(a-b+c)^2=a^2+b^2+c^2-2ab-2bc+2ac$

##### $(a-b-c)^2=a^2+b^2+c^2-2ab+2bc-2ac$

#### Sum of cubes

##### $a^3+b^3=(a+b)(a^2+ab+b^2)$

#### difference of cubes

##### $a^3-b^3=(a-b)(a^2+ab+b^2)$

#### The cube of a binomial

##### $(a+b)^3=a^3+3a^2b+3ab^2+b^3$

##### $(a-b)^3=a^3-3a^2b+3ab^2-b^3$

### Proving identities

#### Developing LHS to reach RHS

#### Developing LHS and RHS to reach the same expression(as A=B and B=C imply A=C)

### Application of identities in expanding, simplifying and evaluating expressions

### Application of identities: Rationalizing the denominator with use of conjugates

### Rational expressions

### Finding the restrictions and simplifying rational expressions

### Adding/subtracting rational expressions

### Multiplying/dividing rational expressions

### Simplifying complex fractions

## Resources

### Identities

#### 1.1 Identities list-updated as we progress

##### $(a+b)^2=(a+b)\times (a+b)=(a+b) \times a+(a+b)\times b=a\times a+b \times a+ a \times b +b \times b=a^2+2ab+b^2$

##### $(a-b)^2=(a-b) \times (a-b)=(a-b)\times a+(a-b)\times (-b)=a \times a-b \times a+a \times(-b)+(-b) \times (-b)=a^2-2ab+b^2$
##### $(a+b)(a-b)=(a+b) \times a-(a+b)\times b=a^2+ab-ab-b^2=a^2-b^2$
##### $(a+b+c)^2=(a+b+c) \times (a+b+c)=(a+b+c) \times a+(a+b+c) \times b+(a+b+c) \times c=a^2+ab+ac+ab+b^2+bc+ac+bc+c^2=a^2+b^2+c^2+2ab+2bc+2ac$
##### $(a+b)^3=(a+b)^2\times(a+b)=(a^2+2ab+b^2) \times a+(a^2+2ab+b^2)\times b=a^3+2a^2b+ab^2+a^2b+2ab^2+b^3=a^3+3a^2b+3ab^2+b^3$
##### $(a-b)^3=(a-b)^2\times (a-b)=(a^2-2ab+b^2)\times a -(a^2-2ab+b^2) \times b=a^3-2a^2b+ab^2-a^2b+2ab^2-b^3=a^3-3a^2b+3ab^2-b^3$
##### $(a-b)(a^2+ab+b^2)=a^3+a^2b+ab^2-a^2b-ab^2-b^3=a^3-b^3$
##### $(a+b)(a^2-ab+b^2)=a^3-a^2b+ab^2+a^2b-ab^2+b^3=a^3+b^3$

#### 1.2 Slides: Identities & applications- Weeks 1-2
##### $(x+3y+5z)^2=x^2+9y^2+25z^2+6xy+10xz+30yz$
##### $(x^2+2x-3)^2=x^4+4x^2+9+4x^3-6x^2-12x=x^4+4x^3-2x^2-12x+9$
##### $(x^2+y^2+y^2)^2=x^4+y^4+z^4+2x^2y^2+2x^2z^2+2y^2z^2$
##### $a^2+b^2+c^2=(a+b+c)^2-2(ab+bc+ca)=10^2-2 \times 24=100-48=52$
##### $16x^2+4y^2+9z^2-16xy+12yz-24zx=(4x)^2+(2y)^2+(3z)^2-2(4x)(2y)+2(2y)(3z)-2(3z)(4x)=(4x-2y-3z)^2$
##### $4c^2-20cd+25d^2=(2c)^2-2(2c)(5d)+(5d)^2=(2c-5d)^2$
##### $a^2+6ab-8ac+9b^2-24bc+16c^2=(a)^2+2(a)(3b)-2(a)(4c)-2(3b)(4c)+(4c)^2=(a+3b-4c)^2$
##### $(2c-5d)^2=4c^2-20cd+25d^2$
##### $(a+3b-4c)^2=a^2+9b^2+16c^2+6ab-8ac-24bc$
##### $(4x+3y)^2-(3x+4y)^2=16x^2+24xy+9y^2-9x^2-24xy-16y^2=7x^2-7y^2=7(x+y)(x-y)=(4x+3y+3x+4y)(4x+3y-3x-4y)=7(x+y)(x-y)$
##### $LHS=(a^2+b^2)(x^2+y^2)=(ax)^2+(ay)^2+(bx)^2+(by)^2,RHS=(ax)^2+(by)^2+2abxy+(ay)^2+(bx)^2-2abxy=(ax)^2+(by)^2+(ay)^2+(bx)^2,LHS=RHS$
##### $(x^2+y^2-z^2)^2-(x^2-y^2+z^2)^2=2x^2(2y^2-2z^2)=4x^2(y-z)(y+z)$
##### $(x+2)^3=x^3+6x^2+12x+8$
##### $(3y-4)^3=27y^3-108y^2+144y-64$
##### $(a+b)^3=a^3+b^3+3ab(a+b),ab=\frac{(a+b)^3-(a^3+b^3)}{3(a+b)}=\frac{8-6}{3 \times 2}=\frac{1}{3}$
##### $(3x+\frac{1}{3}y)^3=27x^3+9x^2y+xy^2+\frac{y^3}{27}$

##### $(5x-\frac{1}{x})^3=125x^3-75x+\frac{15}{x}-\frac{1}{x^3}$

##### $8y^3-\frac{1}{8}=(2y)^3-(\frac{1}{2})^3=(2y-\frac{1}{2})(4y^2+y+\frac{1}{4})$
##### $x^6-64=(x^3+8)(x^3-8)=(x+2)(x^2-2x+4)(x-2)(x^2+2x+4)$
##### $a) xy=\frac{(x-y)^2-(x^2+y^2)}{-2}=\frac{18-10}{-2}=-4,b)\frac{x}{y}+\frac{y}{x}=\frac{x^2+y^2}{xy}=\frac{10}{-4}=-\frac{5}{2}$
##### $\frac{4}{7\sqrt5}=\frac{4\sqrt5}{7\times \sqrt5 \times \sqrt5}=\frac{4\sqrt5}{35}$

##### $\frac{7}{8+2\sqrt3}=\frac{7}{8+2\sqrt3} \times \frac{8-2\sqrt3}{8-2\sqrt3}=\frac{7(8-2\sqrt3)}{52}=\frac{7(4-\sqrt3)}{26}=\frac{28-7\sqrt3}{26}$
##### $\frac{2}{\sqrt2-5\sqrt3}=\frac{2}{\sqrt2-5\sqrt3} \times \frac{\sqrt2+5\sqrt3}{\sqrt2+5\sqrt3}=\frac{2(\sqrt2+5\sqrt3)}{-73}=-\frac{2\sqrt2+10\sqrt3}{73}$
##### $(\sqrt6-\sqrt2)^2-(\sqrt6+\sqrt2)^2=(2\sqrt6)(-2\sqrt2)=-8\sqrt3$
##### $(\sqrt5+2)^3=5\sqrt5+30+12\sqrt5+8=38+17\sqrt5$

##### $(\sqrt5-2\sqrt7)^2-(\sqrt5+\sqrt7)^2=(2\sqrt5-\sqrt7)(-3\sqrt7)=21-6\sqrt35$
##### $(2\sqrt10-3\sqrt2)(2\sqrt10+3\sqrt2)=(2\sqrt10)^2-(3\sqrt2)^2=40-18=22$
##### $(\sqrt5+\sqrt2)^3=5\sqrt5+2\sqrt2+15\sqrt2+6\sqrt5=11\sqrt5+17\sqrt2$
##### $\frac{a-b}{\sqrt a+\sqrt b}=\frac {(\sqrt a+\sqrt b)(\sqrt a-\sqrt b)}{\sqrt a+\sqrt b}=\sqrt a-\sqrt b$
##### $\frac{a-b}{a\sqrt b-b\sqrt a}=\frac{(\sqrt a+\sqrt b)(\sqrt a-\sqrt b)}{\sqrt a \sqrt b (\sqrt a -\sqrt b)}=\frac{\sqrt a+ \sqrt b}{\sqrt a\sqrt b}=\frac{a\sqrt b+b\sqrt a}{ab}$
#### 1.3 Practice: Expanding and simplifying with identities
##### $(x+3)^3$
$$
(x+3)^3
=x^3+9x^2+27x+27
$$
#####  $(1-5x)^3$
$$
(1-5x)^3
=1-15x+75x^2-125x^3
$$
#####  $(2ğ‘¥^2 âˆ’ 3)^3$
$$
(2ğ‘¥^2 âˆ’ 3)^3
=8x^6-36x^4+54x^2-27
$$
#####  $( âˆ’ğ‘¦ âˆ’ 4)^3$
$$
( âˆ’ğ‘¦ âˆ’ 4)^3
=-y^3-12y^2-48y-64
$$
#####  $(âˆ’3 + ğ‘¦)^3$
$$
(âˆ’3 + ğ‘¦)^3
=-27+27y-9y^2+y^3
$$
#####  $(ğ‘¥ âˆ’ 1)(1 + ğ‘¥)$
$$
(ğ‘¥ âˆ’ 1)(1 + ğ‘¥)
=x^2-1
$$
#####  $(3ğ‘¥ âˆ’ 5)(3ğ‘¥ + 5)$
$$
(3ğ‘¥ âˆ’ 5)(3ğ‘¥ + 5)
=9x^2-25
$$
#####  $(4ğ‘ âˆ’ 9ğ‘)(4ğ‘ + 9ğ‘)$
 $$
 (4ğ‘ âˆ’ 9ğ‘)(4ğ‘ + 9ğ‘)
 =16a^2-81b^2
 $$
#####  $(ğ‘¥^2 âˆ’ 4)(ğ‘¥^2 + 4)$

$$
(ğ‘¥^2 âˆ’ 4)(ğ‘¥^2 + 4)
=x^4-16
$$
#####  $(5ğ‘¥^3 + \frac{3y}{2} ) (5ğ‘¥^3 âˆ’ \frac{3y}{2})$
$$
(5ğ‘¥^3 + \frac{3y}{2} ) (5ğ‘¥^3 âˆ’ \frac{3y}{2})
=25x^6-\frac{9y^2}{4}
$$
##### $(11ğ‘¥^2 ğ‘¦ âˆ’ 12ğ‘¤^3 )(11ğ‘¥^2 ğ‘¦ + 12ğ‘¤^3 )$
$$
(11ğ‘¥^2 ğ‘¦ âˆ’ 12ğ‘¤^3 )(11ğ‘¥^2 ğ‘¦ + 12ğ‘¤^3 )
=121x^4y^2-144w^6
$$
#####  $(ğ‘¥ âˆ’ 3)(3 + ğ‘¥)$
$$
(ğ‘¥ âˆ’ 3)(3 + ğ‘¥)
=x^2-9
$$
#####  $(ğ‘¥ âˆ’ ğ‘¦)(âˆ’ğ‘¥ âˆ’ ğ‘¦)$
$$
(ğ‘¥ âˆ’ ğ‘¦)(âˆ’ğ‘¥ âˆ’ ğ‘¦)
=(y-x)(y+x)
=y^2-x^2
$$
#####  $(âˆ’ğ‘¥ + 2)(âˆ’ğ‘¥ âˆ’ 2)$
$$
(âˆ’ğ‘¥ + 2)(âˆ’ğ‘¥ âˆ’ 2)
=(x-2)(x+2)
=x^2-4
$$
#####  $(\sqrt3 âˆ’ \sqrt2)(\sqrt3 + \sqrt2)$
$$
(\sqrt3 âˆ’ \sqrt2)(\sqrt3 + \sqrt2)
=3-2
=1
$$
#####  $(1 âˆ’ 2\sqrt3) (1 + 2\sqrt3)$
$$
(1 âˆ’ 2\sqrt3) (1 + 2\sqrt3)
=1-12
=-11
$$
##### $\frac{1}{(2âˆ’\sqrt3)(2+\sqrt3)}$
$$
\frac{1}{(2âˆ’\sqrt3)(2+\sqrt3)}
=\frac{1}{4-3} 
=1
$$
##### $\frac{2}{(3+\sqrt5)}$
$$
\frac{2}{(3+\sqrt5)}
=\frac{2}{(3+\sqrt5)} \times \frac{(3-\sqrt5)}{(3-\sqrt5)}
=\frac{2(3-\sqrt5)}{9-5}
=\frac{3-\sqrt5}{2}
$$
##### $\frac{1}{(1âˆ’2\sqrt3)}$
$$
\frac{1}{(1âˆ’2\sqrt3)}
=\frac{1}{1âˆ’2\sqrt3} \times \frac{1+2\sqrt3}{1+2\sqrt3}
=\frac{1+2\sqrt3}{1-12}
=-\frac{1+2\sqrt3}{11}
$$

#####  $(ğ‘¥ âˆ’ 1)(ğ‘¥ + 1)(ğ‘¥^2 + 1)(ğ‘¥^4 + 1)$
$$
\begin{aligned}
&(ğ‘¥ âˆ’ 1)(ğ‘¥ + 1)(ğ‘¥^2 + 1)(ğ‘¥^4 + 1) \\
=&(x^2-1)(x^2+1)(x^4+1) \\
=&(x^4-1)(x^4+1) \\
=&x^8-1
\end{aligned}
$$
#####  $(ğ‘¥ âˆ’ 2)^2 (ğ‘¥ + 2)^2 (ğ‘¥^2 + 4)^2$
$$
\begin{aligned}
&(ğ‘¥ âˆ’ 2)^2 (ğ‘¥ + 2)^2 (ğ‘¥^2 + 4)^2 \\
=&(x^2-4)^2(x^2+4)^2 \\
=&(x^4-16)^2 \\
=&x^8-32x^4+256 \\
\end{aligned}
$$
##### Let $ğ‘ƒ = (2ğ‘¥ âˆ’ 1)^2 âˆ’ 3(ğ‘¥ âˆ’ 2)(ğ‘¥ + 2) + 4ğ‘¥ âˆ’ 13.$
Find the value of $ğ´ = \sqrtğ‘ƒ$, when $ğ‘¥ = 2022$.
$$
\begin{aligned}
ğ‘ƒ &= (2ğ‘¥ âˆ’ 1)^2 âˆ’ 3(ğ‘¥ âˆ’ 2)(ğ‘¥ + 2) + 4ğ‘¥ âˆ’ 13 \\
&=4x^2-4x+1-3x^2+12+4x-13 \\
&=x^2 \\
A&=\sqrt P=|x|=2022
\end{aligned}
$$
#####  $(ğ‘¥ + 3)(ğ‘¥^2 âˆ’ 3ğ‘¥ + 9)$
$$
\begin{aligned}
&(ğ‘¥ + 3)(ğ‘¥^2 âˆ’ 3ğ‘¥ + 9) \\
=&x^3-3x^2+9x+3x^2-9x+27 \\
=&x^3+27
\end{aligned}
$$
#####  $(2ğ‘¦ âˆ’ 1)(4ğ‘¦^2 + 2ğ‘¦ + 1)$
$$
\begin{aligned}
&(2ğ‘¦ âˆ’ 1)(4ğ‘¦^2 + 2ğ‘¦ + 1) \\
=&8y^3+4y^2+2y-4y^2-2y-1 \\
=&8y^3-1
\end{aligned}
$$

#####  $(3ğ‘¥ + ğ‘¦ + 2)^2$
$$
\begin{aligned}
&(3ğ‘¥ + ğ‘¦ + 2)^2 \\
&=9x^2+y^2+4+6xy+12x+4y \\
&=9x^2+6xy+y^2+12x+4y+4
\end{aligned}
$$
#####  $(ğ‘¥^2 âˆ’ 3ğ‘¥ âˆ’ 1)^2$
$$
\begin{aligned}
&(ğ‘¥^2 âˆ’ 3ğ‘¥ âˆ’ 1)^2 \\
=&x^4+9x^2+1-6x^3-2x^2+6x \\
=&x^4-6x^3+7x^2+6x+1\\
\\
&(ğ‘¥^2 âˆ’ 3ğ‘¥ + 1)^2 \\
=&x^4+9x^2+1-6x^3+2x^2-6x \\
=&x^4-6x^3+11x^2-6x+1 \\
&\text {(The teacher did like this, because copying the question incorrectly)} 
\end{aligned}
$$
#####  $(1 âˆ’ ğ‘¥)(3 âˆ’ ğ‘¥)$
$$
\begin{aligned}
&(1 âˆ’ ğ‘¥)(3 âˆ’ ğ‘¥) \\
=&3-x-3x+x^2 \\
=&x^2-4x+3
\end{aligned}
$$
#####  $(2ğ‘¥ + 5)(3ğ‘¥ âˆ’ 1) âˆ’ (3ğ‘¥ âˆ’ 2)(2ğ‘¥ + 7)$
$$
\begin{aligned}
&(2ğ‘¥ + 5)(3ğ‘¥ âˆ’ 1) âˆ’ (3ğ‘¥ âˆ’ 2)(2ğ‘¥ + 7) \\
=&(6x^2+13x-5)-(6x^2+17x-14) \\
=&-4x+9 \\
&\text {(The teacher made a mistake)} 
\end{aligned}
$$
##### Let $(ğ‘ + ğ‘) = âˆ’1$ and $ğ‘ğ‘ = âˆ’2$. Evaluate:
##### $ğ‘^2 + ğ‘^2$
$$
\begin{aligned}
&a^2+b^2 \\
=&(a+b)^2-2ab \\
=&(-1)^2-2\times (-2) \\
=&5
\end{aligned}
$$
##### $ğ‘^3 + ğ‘^3$
$$
\begin{aligned}
&a^3+b^3 \\
=&(a+b)^3-3ab(a+b) \\
=&(-1)^3-3(-2)(-1) \\
=&-7
\end{aligned}
$$
#####  $(ğ‘ âˆ’ ğ‘)^2$
$$
\begin{aligned}
&(a-b)^2 \\
=&(a+b)^2-4ab \\
=&(-1)^2-4(-2) \\
=&9

\end{aligned}
$$

#####  $99^2$
$$
\begin{aligned}
&99^2 \\
=&(100-1)^2 \\
=&100^2-2(1)(100)+1^1 \\
=&10,000-200+1 \\
=&9801
\end{aligned}
$$
#####  $1002 â‹… 998$
$$
\begin{aligned}
&1002 \times 998 \\
=&(1,000+2)(1,000-2) \\
=&1,000^2-2^2 \\
=&1,000,000-4 \\
=&999,996
\end{aligned}
$$
#####  Show that $(ğ‘ + 2)^2 âˆ’ 4(ğ‘ + 1) = ğ‘^2$
$$
\begin{aligned}
&LHS=a^2+4a+4-4a-4=a^2\\
&RHS=a^2 \\
&LHS=RHS
\end{aligned}
$$
#####  Evaluate $ğ´ = \sqrt{1002^2 âˆ’ 4004}$
$$
\begin{aligned}
A&=\sqrt{1002^2-4004} \\
&=\sqrt{(1000+2)^2-2(1000)(2)-2^2} \\
&=\sqrt{1000^2} \\
&=1000

\end{aligned}
$$





#### 1.4 More practice on expanding and Identities
#####  $(2ğ‘ + 4ğ‘)^2$
$$
\begin{aligned}
&(2a+4b)^2 \\
=&4a^2+16ab+16b^2
\end{aligned}
$$
#####  $2(3ğ‘¥ + 4)^2 âˆ’ (4ğ‘¥ + 3)^2$
$$
\begin{aligned}
&2(3x+4)^2-(4x+3)^2 \\
=&2(9x^2+24x+16)-(16x^2+24x+9) \\
=&(18x^2+48x+32)-(16x^2+24x+9) \\
=&2x^2+24x+23
\end{aligned}
$$
#####  $(7ğ‘¥ âˆ’ 1)^2 âˆ’ 5(ğ‘¥ âˆ’ 2)^2$
$$
\begin{aligned}
&(7ğ‘¥ âˆ’ 1)^2 âˆ’ 5(ğ‘¥ âˆ’ 2)^2 \\
=&(49x^2-14x+1)-(5x^2-20x+20) \\
=&44x^2+6x-19
\end{aligned}
$$
#####  $(ğ‘ + 3ğ‘¥ + 2)^2$
$$
\begin{aligned}
&(a+3x+2)^2 \\
=&a^2+9x^2+4+6ax+4a+12x \\
=&a^2+6ax+9x^2+4a+12x+4


\end{aligned}
$$
#####  $(ğ‘¥ + 1)(4 âˆ’ ğ‘¥ âˆ’ ğ‘¥^2)$
$$
\begin{aligned}
&(x+1)(4-x-x^2) \\
=&4x-x^2-x^3+4-x-x^2 \\
=&-x^3-2x^2+3x+4
\end{aligned}
$$
#####  $(ğ‘¥ âˆ’ ğ‘¦)^3$
$$
\begin{aligned}
&(x-y)^3 \\
=&x^3-3x^2y+3xy^2-y^3 
\end{aligned}
$$
#####  $\left(1 âˆ’ \frac{3}{ğ‘¥}\right)^2+\left(\frac{2}{ğ‘¥}âˆ’ 1\right)^2$
$$ 
\begin{aligned} 
&\left(1-\frac{3}{x}\right)^2 + \left(\frac{2}{x}-1\right)^2 \\ 
=& \left(1-\frac{6}{x}+\frac{9}{x^2}\right) + \left(\frac{4}{x^2}- \frac{4}{x}+1\right) \\ 
=& \frac{13}{x^2} - \frac{10}{x} + 2 
\end{aligned} 
$$
#####  $3\left(ğ‘¥ + \frac{4}{ğ‘¥}\right)^2$
$$
\begin{aligned}
&3\left(x+\frac{4}{x}\right)^2 \\
=&3\left(x^2+8+\frac{16}{x^2}\right) \\
=&3x^2+24+\frac{48}{x^2}
\end{aligned}
$$

#####  $(ğ‘ + ğ‘)^2 + (ğ‘ âˆ’ ğ‘)^2 = 2ğ‘^2 + 2ğ‘^2$

$$
\begin{aligned}
LHS=a^2+2ab+b^2+a^2-2ab+b^2=2a^2+2b^2=RHS
\end{aligned}
$$
#####  $(ğ‘ + ğ‘)^2 âˆ’ (ğ‘ âˆ’ ğ‘)^2 = 4ğ‘ğ‘$
$$
\begin{aligned}
LHS=(a^2+2ab+b^2)-(a^2-2ab+b^2)=4ab=RHS
\end{aligned}
$$
#####  $ğ‘^4 âˆ’ ğ‘^4 = (ğ‘^2 + ğ‘^2)(ğ‘ âˆ’ ğ‘)(ğ‘ + ğ‘)$
$$
\begin{aligned}
LHS=(a^2+b^2)(a^2-b^2)=(a^2+b^2)(a+b)(a-b)=RHS
\end{aligned}
$$
#####  $2(2ğ‘¥ âˆ’ 1)^3 âˆ’ (ğ‘¥ âˆ’ 2)(4ğ‘¥ + 1)^2 = 27ğ‘¥$
$$
\begin{aligned}
&2(2x-1)^3-(x-2)(4x+1)^2 \\
=&2(8x^3-12x^2+6x-1)-(x-2)(16x^2+8x+1) \\
=&(16x^3-24x^2+12x-2)-(16x^3-24x^2-15x-2) \\
=&27x
\end{aligned}
$$
#####  $\left(ğ‘¥ +\frac{1}{ğ‘¥}\right)^2âˆ’ \left(ğ‘¥ âˆ’\frac{1}{ğ‘¥}\right)^2= 4$
$$
\begin{aligned}
&\left(x+\frac{1}{x}\right)^2-\left(x-\frac{1}{x}\right)^2 \\
=&\left(x^2+2+\frac{1}{x^2}\right)-\left(x^2-2+\frac{1}{x^2}\right) \\
=& 4
\end{aligned}
$$
#####  $(4ğ‘¥ + 3ğ‘¦)^2 âˆ’ (3ğ‘¥ + 4ğ‘¦)^2 = 7(ğ‘¥ + ğ‘¦)(ğ‘¥ âˆ’ ğ‘¦)$
$$
\begin{aligned}
&(4x+3y)^2-(3x+4y)^2 \\
=&(16x^2+24xy+9y^2)-(9x^2+24xy+16y^2)\\
=&7x^2-7y^2 \\
=&7(x+y(x-y))
\end{aligned}
$$
#####  $(2ğ‘¥ + ğ‘¦)^2 âˆ’ (ğ‘¥ + 2ğ‘¦)^2 = 3(ğ‘¥ + ğ‘¦)(ğ‘¥ âˆ’ ğ‘¦)$
$$
\begin{aligned}
&(2x+y)^2-(x+2y)^2 \\
=&(4x^2+4xy+y^2)-(x^2+4xy+4y^2) \\
=&3x^2-3y^2 \\
=&3(x+y)(x-y)
\end{aligned}
$$
#####  $(2ğ‘ + ğ‘)^2 + ğ‘^2 = 2[ğ‘^2 + (ğ‘ + ğ‘)^2]$
$$
\begin{aligned}
&LHS \\
=&(2a+b)^2+b^2 \\
=&4a^2+4ab+b^2+b^2 \\
=&4a^2+4ab+2b^2 \\
\\
&RHS \\
=&2[a^2+(a+b)^2]\\
=&2(a^2+a^2+2ab+b^2) \\
=&4a^2+4ab+2b^2 \\
\\
&LHS=RHS
\end{aligned}
$$
#####  $(ğ‘^2 + ğ‘^2)(ğ‘¥^2 + ğ‘¦^2) = (ğ‘ğ‘¥ + ğ‘ğ‘¦)^2 + (ğ‘ğ‘¦ âˆ’ ğ‘ğ‘¥)^2$
$$
\begin{aligned}
LHS=&a^2x^2+a^2y^2+b^2x^2+b^2y^2 \\

RHS=&a^2x^2+b^2y^2+2abxy+a^2y^2+b^xy^2-2abxy \\
=&a^2x^2+b^2y^2+a^2y^2+b^2x^2 \\
\\
LHS&=RHS
\end{aligned}
$$
##### It is given that $ğ‘¥^2 + ğ‘¦^2 = 8$ and $ğ‘¥ğ‘¦ = âˆ’3$ 
Find the value of 
a. $(ğ‘¥ + ğ‘¦)^2$ 
$$(x+y)^2=x^2+y^2+2xy=8+2(-3)=2$$
b. $(ğ‘¥ âˆ’ ğ‘¦)^2$ 
$$(x-y)^2=x^2+y^2-2xy=8-2(-3)=14$$
c. $ğ‘¥^3 + ğ‘¦^3$
$$x^3+y^3=(x+y)(x^2-xy+y^2)=(\pm \sqrt2)(8-(-3))=\pm11\sqrt2$$
##### It is given that $ğ‘¥ + \frac{1}{ğ‘¥} = 4$. Find the value of $ğ‘¥^2 + \frac{1}{ğ‘¥^2}$ .
$$
\begin{aligned}
\left(x+\frac{1}{x}\right)^2=x^2+\frac{1}{x^2}+2 \\
x^2+\frac{1}{x^2}=\left(x+\frac{1}{x}\right)^2-2=4^2-2=14
\end{aligned}
$$
##### Let $ğ‘ + ğ‘ + ğ‘ = 0$, Show that $ğ‘^3 + ğ‘^3 + ğ‘^3 = 3ğ‘ğ‘$
$$
\begin{aligned}
&(a+b+c)^3 \\
=&(a+b+c)(a+b+c)^2 \\
=&(a+b+c)(a^2+b^2+c^2+2ab+2ac+2bc) \\
=&a^3+ab^2+ac^2+2a^2b+2a^2c+2abc \\
&+a^2b+b^3+bc^2+2ab^2+2abc+2b^2c \\
&+a^2c+b^2c+c^3+2abc+2ac^2+2bc^2 \\
=&a^3+b^3+c^3+3a^2b+3a^2c+3ab^2+3ac^2+3b^2c+3bc^2+6abc \\
=&a^3+b^3+c^3+3(a^2b+ab^2+b^2c+bc^2+c^2a+ca^2)+6abc \\
=&a^3+b^3+c^3+3(a^2b+ab^2+abc+b^2c+bc^2+abc+c^2a+ca^2+abc)-3abc \\
=&a^3+b^3+c^3+3(a+b+c)(ab+bc+ca)-3abc \\
&\because a+b+c=0 \\
&\therefore 0=a^3+b^3+c^3-3abc \\
&a^3+b^3+c^3=3abc \\
\\
&\because a+b+c=0 \\
&\therefore c=-a-b=-(a+b) \\
&a^3+b^3+c^3 \\
=&a^3+b^3+(-a-b)^3 \\
=&a^3+b^3-(a^3+b^3+3a^2b+3ab^2) \\
=&-3a^2b-3ab^2 \\
=&-3ab(a+b) \\
=&3abc
\end{aligned}$$
#####  $(\sqrt 2 âˆ’ \sqrt 8)^2$
$$=(\sqrt2-\sqrt8)^2=(\sqrt2-2\sqrt2)^2=(-\sqrt2)^2=2$$
#####  $(\sqrt 7 + 3\sqrt 5)^2$
$$(\sqrt7+3\sqrt5)^2=7+45+6\sqrt{35}=52+6\sqrt{35}$$
##### $\frac{(\sqrt 3âˆ’2\sqrt 5)^2}{\sqrt {15}}$
$$\frac{(\sqrt3-2\sqrt5)^2}{\sqrt{15}}=\frac{3+20-4\sqrt{15}}{\sqrt{15}}=\frac{23\sqrt{15}-60}{15}=\frac{23\sqrt{15}}{15}-4$$
#####  $\frac{(3âˆ’\sqrt 2)^2}{\sqrt 2}$
$$\frac{(3âˆ’\sqrt 2)^2}{\sqrt 2}=\frac{11-6\sqrt2}{\sqrt2}=\frac{11\sqrt2-12}{2}=\frac{11\sqrt2}{2}-6$$
##### $\frac{\sqrt 2âˆ’3\sqrt 3}{\sqrt 3}$
$$\frac{\sqrt2-3\sqrt3}{\sqrt3}=\frac{\sqrt6-9}{3}=\frac{\sqrt6}{3}-3$$
#####  $\frac{4}{3+\sqrt 5}$
$$\frac{4}{3+\sqrt5}=\frac{12-4\sqrt5}{4}=3-\sqrt5$$
##### $\frac{3âˆ’\sqrt 6}{3+\sqrt 6}$
$$\frac{3âˆ’\sqrt 6}{3+\sqrt 6}=\frac{15-6\sqrt6}{3}=5-2\sqrt6$$
#####  $\frac{\sqrt 14âˆ’2}{\sqrt 7âˆ’\sqrt 2}$
$$\frac{\sqrt 14âˆ’2}{\sqrt 7âˆ’\sqrt 2}=\frac{\sqrt 14âˆ’2}{\sqrt 7âˆ’\sqrt 2}\times \frac{\sqrt 7+\sqrt 2}{\sqrt 7+\sqrt 2}=\frac{7\sqrt2+2\sqrt7-2\sqrt7-2\sqrt2}{5}=\sqrt2$$
#### 1.5 Practice on trinomial squares: with answers

#### 1.6 Rationalizing denominators-with answers

#### Assignments

##### Assignment 1.1-Identities-due Sep 12

##### Assignment 1.2-Identities and more-due Sep 16

##### Assignment 1.3-Sum/difference of cubes & rationalizing denominators

##### Assignment 1.4-Radicals and identities-due Sep 23

### Factoring

#### 1.7 Practice: Sum/difference of cubes-with answers

#### 1.8 Practice: Sum/difference of cubes 2-with answers

#### 1.9 Sum/difference of cubes incl. change of variable: answers at the end

#### 1.10 Combinations of GCF with other methods: answers at the end

#### 1.11 Quadratics that include square roots-with answers

#### 1.12 Advanced factoring by common factor: with answers

#### 1.13 Slides: Factoring -Weeks 3-4

#### Assignments

##### Assignment 1.5 Factoring

##### Assignment 1.6 Identities & Factoring

##### Test 2-Periods 6 & 8-October 21

### Rational Expressions

#### 1.14 Slides: Rational expressions Weeks 5-6

#### 1.15 Video: Multiplying rational expressions

#### 1.16 Video: Dividing rational expressions

#### 1.17 Exercises on multiplying and dividing rational expressions-with answers

#### 1.18 More Exercises on multiplying and dividing rational expressions

#### 1.19 Video: Finding the LCM of rational expressions

#### 1.20 Video: Adding and subtracting rational expressions

#### 1.21 Exercises on Adding & Subtracting rational expressions-with answers

#### 1.22 Exercises on Complex fractions-with answers

#### 1.23 Revision on factoring and identities (Task 2 of HW 1.9)

#### 1.24 Revision of rational expressions-wtih answers

#### Assignments

##### Assignment 1.7 Rational expressions-Period 8-due Oct 2

##### Assignment 1.8-Rational expressions-due Oct 10

##### Assignment 1.9-Rational expressions & Review-due Oct 14

##### Assignment 1.10 Complex fractions & Delta math-due Oct 17

##### Test 2-Periods 6 & 8-October 21

## Assignments